SeparationLogic/SeparationLogic.v
@@ -5,18 +5,103 @@ Require Import Logic.MinimunLogic.MinimunLogic.
 Require Import Logic.MinimunLogic.ContextProperty.
 Require Import Logic.PropositionalLogic.Syntax.
 Require Import Logic.PropositionalLogic.IntuitionisticPropositionalLogic.
+Require Import Logic.PropositionalLogic.GodelDummettLogic.
+Require Import Logic.PropositionalLogic.ClassicalPropositionalLogic.
 Require Import Logic.SeparationLogic.Syntax.
 
 Local Open Scope logic_base.
 Local Open Scope PropositionalLogic.
 Local Open Scope SeparationLogic.
 
-Class SeparationLogic (L: Language) {nL: NormalLanguage L} {pL: PropositionalLanguage L} {SL: SeparationLanguage L} (Gamma: ProofTheory L) {mpGamma: MinimunPropositionalLogic L Gamma} {ipGamma: IntuitionisticPropositionalLogic L Gamma} := {
+Class SeparationLogic (L: Language) {nL: NormalLanguage L} {pL: PropositionalLanguage L} {sL: SeparationLanguage L} (Gamma: ProofTheory L) {nGamma: NormalProofTheory L Gamma} {mpGamma: MinimunPropositionalLogic L Gamma} {ipGamma: IntuitionisticPropositionalLogic L Gamma} := {
   sepcon_comm: forall x y, |-- x * y --> y * x;
   sepcon_assoc: forall x y z, |-- x * (y * z) <--> (x * y) * z;
   wand_sepcon_adjoin: forall x y z, |-- x * y --> z <-> |-- x --> (y -* z);
   sepcon_mono: forall x1 x2 y1 y2, |-- x1 --> x2 -> |-- y1 --> y2 -> |-- (x1 * y1) --> (x2 * y2)
 }.
+
+Class UnitarySeparationLogic (L: Language) {nL: NormalLanguage L} {pL: PropositionalLanguage L} {sL: SeparationLanguage L} {usL: UnitarySeparationLanguage L} (Gamma: ProofTheory L) {nGamma: NormalProofTheory L Gamma} {mpGamma: MinimunPropositionalLogic L Gamma} {ipGamma: IntuitionisticPropositionalLogic L Gamma} {sGamma: SeparationLogic L Gamma} := {
+  sepcon_emp: forall x, |-- x * emp <--> x
+}.
+
+Class GarbageCollectSeparationLogic (L: Language) {nL: NormalLanguage L} {pL: PropositionalLanguage L} {sL: SeparationLanguage L} (Gamma: ProofTheory L) {nGamma: NormalProofTheory L Gamma} {mpGamma: MinimunPropositionalLogic L Gamma} {ipGamma: IntuitionisticPropositionalLogic L Gamma} {sGamma: SeparationLogic L Gamma} := {
+  sepcon_elim1: forall x y, |-- x * y --> x
+}.
+
+Lemma derivable_sepcon_comm: forall {L: Language} {nL: NormalLanguage L} {pL: PropositionalLanguage L} {sL: SeparationLanguage L} {Gamma: ProofTheory L} {nGamma: NormalProofTheory L Gamma} {mpGamma: MinimunPropositionalLogic L Gamma} {ipGamma: IntuitionisticPropositionalLogic L Gamma} {sGamma: SeparationLogic L Gamma} (Phi: context) (x y: expr),
+  Phi |-- x * y --> y * x.
+Proof.
+  intros.
+  pose proof sepcon_comm x y.
+  apply deduction_weaken0; auto.
+Qed.
+
+Lemma derivable_sepcon_assoc: forall {L: Language} {nL: NormalLanguage L} {pL: PropositionalLanguage L} {sL: SeparationLanguage L} {Gamma: ProofTheory L} {nGamma: NormalProofTheory L Gamma} {mpGamma: MinimunPropositionalLogic L Gamma} {ipGamma: IntuitionisticPropositionalLogic L Gamma} {sGamma: SeparationLogic L Gamma} (Phi: context) (x y z: expr),
+  Phi |-- x * (y * z) <--> (x * y) * z.
+Proof.
+  intros.
+  pose proof sepcon_assoc x y z.
+  apply deduction_weaken0; auto.
+Qed.
+
+Lemma derivable_sepcon_emp: forall {L: Language} {nL: NormalLanguage L} {pL: PropositionalLanguage L} {sL: SeparationLanguage L} {usL: UnitarySeparationLanguage L} {Gamma: ProofTheory L} {nGamma: NormalProofTheory L Gamma} {mpGamma: MinimunPropositionalLogic L Gamma} {ipGamma: IntuitionisticPropositionalLogic L Gamma} {sGamma: SeparationLogic L Gamma} {usGamma: UnitarySeparationLogic L Gamma} (Phi: context) (x: expr),
+  Phi |-- x * emp <--> x.
+Proof.
+  intros.
+  pose proof sepcon_emp x.
+  apply deduction_weaken0; auto.
+Qed.
+
+Lemma deduction_sepcon_comm: forall {L: Language} {nL: NormalLanguage L} {pL: PropositionalLanguage L} {sL: SeparationLanguage L} {Gamma: ProofTheory L} {nGamma: NormalProofTheory L Gamma} {mpGamma: MinimunPropositionalLogic L Gamma} {ipGamma: IntuitionisticPropositionalLogic L Gamma} {sGamma: SeparationLogic L Gamma} (Phi: context) (x y: expr),
+  Phi |-- x * y <-> Phi |-- y * x.
+Proof.
+  intros.
+  pose proof derivable_sepcon_comm Phi x y.
+  pose proof derivable_sepcon_comm Phi y x.
+  split; intros; eapply deduction_modus_ponens; eauto.
+Qed.
+
+Lemma deduction_sepcon_assoc: forall {L: Language} {nL: NormalLanguage L} {pL: PropositionalLanguage L} {sL: SeparationLanguage L} {Gamma: ProofTheory L} {nGamma: NormalProofTheory L Gamma} {mpGamma: MinimunPropositionalLogic L Gamma} {ipGamma: IntuitionisticPropositionalLogic L Gamma} {sGamma: SeparationLogic L Gamma} (Phi: context) (x y z: expr),
+  Phi |-- x * (y * z) <-> Phi |-- (x * y) * z.
+Proof.
+  intros.
+  pose proof derivable_sepcon_assoc Phi x y z.
+  pose proof deduction_andp_elim1 _ _ _ H.
+  pose proof deduction_andp_elim2 _ _ _ H.
+  split; intros; eapply deduction_modus_ponens; eauto.
+Qed.
+
+Lemma derivable_sepcon_elim1: forall {L: Language} {nL: NormalLanguage L} {pL: PropositionalLanguage L} {sL: SeparationLanguage L} {Gamma: ProofTheory L} {nGamma: NormalProofTheory L Gamma} {mpGamma: MinimunPropositionalLogic L Gamma} {ipGamma: IntuitionisticPropositionalLogic L Gamma} {sGamma: SeparationLogic L Gamma} {gcsGamma: GarbageCollectSeparationLogic L Gamma} (Phi: context) (x y: expr),
+  Phi |-- x * y --> x.
+Proof.
+  intros.
+  pose proof sepcon_elim1 x y.
+  apply deduction_weaken0; auto.
+Qed.
+
+Lemma derivable_sepcon_elim2: forall {L: Language} {nL: NormalLanguage L} {pL: PropositionalLanguage L} {sL: SeparationLanguage L} {Gamma: ProofTheory L} {nGamma: NormalProofTheory L Gamma} {mpGamma: MinimunPropositionalLogic L Gamma} {ipGamma: IntuitionisticPropositionalLogic L Gamma} {sGamma: SeparationLogic L Gamma} {gcsGamma: GarbageCollectSeparationLogic L Gamma} (Phi: context) (x y: expr),
+  Phi |-- x * y --> y.
+Proof.
+  intros.
+  intros.
+  pose proof derivable_sepcon_elim1 Phi y x.
+  eapply deduction_impp_trans; eauto.
+  apply deduction_weaken0.
+  apply sepcon_comm.
+Qed.
+
+Lemma derivable_emp: forall {L: Language} {nL: NormalLanguage L} {pL: PropositionalLanguage L} {sL: SeparationLanguage L} {usL: UnitarySeparationLanguage L} {Gamma: ProofTheory L} {nGamma: NormalProofTheory L Gamma} {mpGamma: MinimunPropositionalLogic L Gamma} {ipGamma: IntuitionisticPropositionalLogic L Gamma} {sGamma: SeparationLogic L Gamma} {usGamma: UnitarySeparationLogic L Gamma} {gcsGamma: GarbageCollectSeparationLogic L Gamma} (Phi: context) (x y: expr),
+  Phi |-- emp.
+Proof.
+  intros.
+  pose proof derivable_sepcon_elim2 Phi TT emp.
+  pose proof derivable_sepcon_emp Phi TT.
+  apply deduction_andp_elim2 in H0.
+  pose proof derivable_impp_refl Phi FF.
+  pose proof deduction_modus_ponens _ _ _ H1 H0.
+  pose proof deduction_modus_ponens _ _ _ H2 H.
+  auto.
+Qed.
 
 Module SeparationLogic.
 Section SeparationLogic.
@@ -26,7 +111,7 @@ Context (Var: Type).
 Instance L: Language := SeparationLanguage.L Var.
 Instance nL: NormalLanguage L := SeparationLanguage.nL Var.
 Instance pL: PropositionalLanguage L := SeparationLanguage.pL Var.
-Instance SL: SeparationLanguage L := SeparationLanguage.SL Var.
+Instance SL: SeparationLanguage L := SeparationLanguage.sL Var.
 
 Inductive provable: expr -> Prop :=
 | modus_ponens: forall x y, provable (x --> y) -> provable x -> provable y
@@ -82,4 +167,323 @@ Qed.
 
 End SeparationLogic.
 End SeparationLogic.
+
+Module ReynoldsLogic.
+Section ReynoldsLogic.
+
+Context (Var: Type).
+
+Instance L: Language := SeparationLanguage.L Var.
+Instance nL: NormalLanguage L := SeparationLanguage.nL Var.
+Instance pL: PropositionalLanguage L := SeparationLanguage.pL Var.
+Instance SL: SeparationLanguage L := SeparationLanguage.sL Var.
+
+Inductive provable: expr -> Prop :=
+| modus_ponens: forall x y, provable (x --> y) -> provable x -> provable y
+| axiom1: forall x y, provable (x --> (y --> x))
+| axiom2: forall x y z, provable ((x --> y --> z) --> (x --> y) --> (x --> z))
+| andp_intros: forall x y, provable (x --> y --> x && y)
+| andp_elim1: forall x y, provable (x && y --> x)
+| andp_elim2: forall x y, provable (x && y --> y)
+| orp_intros1: forall x y, provable (x --> x || y)
+| orp_intros2: forall x y, provable (y --> x || y)
+| orp_elim: forall x y z, provable ((x --> z) --> (y --> z) --> (x || y --> z))
+| falsep_elim: forall x, provable (FF --> x)
+| sepcon_comm: forall x y, provable (x * y --> y * x)
+| sepcon_assoc: forall x y z, provable (x * (y * z) <--> (x * y) * z)
+| wand_sepcon_adjoint1: forall x y z, provable (x * y --> z) -> provable (x --> (y -* z))
+| wand_sepcon_adjoint2: forall x y z, provable (x --> (y -* z)) -> provable (x * y --> z)
+| sepcon_mono: forall x1 x2 y1 y2, provable (x1 --> x2) -> provable (y1 --> y2) -> provable ((x1 * y1) --> (x2 * y2))
+| sepcon_elim1: forall x y, provable (x * y --> x).
+
+Instance G: ProofTheory L := Build_AxiomaticProofTheory provable.
+
+Instance nG: NormalProofTheory L G := Build_nAxiomaticProofTheory provable.
+
+Instance mpG: MinimunPropositionalLogic L G.
+Proof.
+  constructor.
+  + apply modus_ponens.
+  + apply axiom1.
+  + apply axiom2.
+Qed.
+
+Instance ipG: IntuitionisticPropositionalLogic L G.
+Proof.
+  constructor.
+  + apply andp_intros.
+  + apply andp_elim1.
+  + apply andp_elim2.
+  + apply orp_intros1.
+  + apply orp_intros2.
+  + apply orp_elim.
+  + apply falsep_elim.
+Qed.
+
+Instance sG: SeparationLogic L G.
+Proof.
+  constructor.
+  + apply sepcon_comm.
+  + apply sepcon_assoc.
+  + intros; split.
+    - apply wand_sepcon_adjoint1.
+    - apply wand_sepcon_adjoint2.
+  + apply sepcon_mono.
+Qed.
+
+Instance gcsG: GarbageCollectSeparationLogic L G.
+Proof.
+  constructor.
+  apply sepcon_elim1.
+Qed.
+
+End ReynoldsLogic.
+End ReynoldsLogic.
+
+Module OHearnLogic.
+Section OHearnLogic.
+
+Context (Var: Type).
+
+Instance L: Language := UnitarySeparationLanguage.L Var.
+Instance nL: NormalLanguage L := UnitarySeparationLanguage.nL Var.
+Instance pL: PropositionalLanguage L := UnitarySeparationLanguage.pL Var.
+Instance SL: SeparationLanguage L := UnitarySeparationLanguage.sL Var.
+Instance usL: UnitarySeparationLanguage L := UnitarySeparationLanguage.usL Var.
+
+Inductive provable: expr -> Prop :=
+| modus_ponens: forall x y, provable (x --> y) -> provable x -> provable y
+| axiom1: forall x y, provable (x --> (y --> x))
+| axiom2: forall x y z, provable ((x --> y --> z) --> (x --> y) --> (x --> z))
+| andp_intros: forall x y, provable (x --> y --> x && y)
+| andp_elim1: forall x y, provable (x && y --> x)
+| andp_elim2: forall x y, provable (x && y --> y)
+| orp_intros1: forall x y, provable (x --> x || y)
+| orp_intros2: forall x y, provable (y --> x || y)
+| orp_elim: forall x y z, provable ((x --> z) --> (y --> z) --> (x || y --> z))
+| falsep_elim: forall x, provable (FF --> x)
+| excluded_middle: forall x, provable (x || ~~ x)
+| sepcon_comm: forall x y, provable (x * y --> y * x)
+| sepcon_assoc: forall x y z, provable (x * (y * z) <--> (x * y) * z)
+| wand_sepcon_adjoint1: forall x y z, provable (x * y --> z) -> provable (x --> (y -* z))
+| wand_sepcon_adjoint2: forall x y z, provable (x --> (y -* z)) -> provable (x * y --> z)
+| sepcon_mono: forall x1 x2 y1 y2, provable (x1 --> x2) -> provable (y1 --> y2) -> provable ((x1 * y1) --> (x2 * y2))
+| sepcon_emp: forall x, provable (x * emp <--> x).
+
+Instance G: ProofTheory L := Build_AxiomaticProofTheory provable.
+
+Instance nG: NormalProofTheory L G := Build_nAxiomaticProofTheory provable.
+
+Instance mpG: MinimunPropositionalLogic L G.
+Proof.
+  constructor.
+  + apply modus_ponens.
+  + apply axiom1.
+  + apply axiom2.
+Qed.
+
+Instance ipG: IntuitionisticPropositionalLogic L G.
+Proof.
+  constructor.
+  + apply andp_intros.
+  + apply andp_elim1.
+  + apply andp_elim2.
+  + apply orp_intros1.
+  + apply orp_intros2.
+  + apply orp_elim.
+  + apply falsep_elim.
+Qed.
+
+Instance cpG: ClassicalPropositionalLogic L G.
+Proof.
+  constructor.
+  apply excluded_middle.
+Qed.
+
+Instance sG: SeparationLogic L G.
+Proof.
+  constructor.
+  + apply sepcon_comm.
+  + apply sepcon_assoc.
+  + intros; split.
+    - apply wand_sepcon_adjoint1.
+    - apply wand_sepcon_adjoint2.
+  + apply sepcon_mono.
+Qed.
+
+Instance usG: UnitarySeparationLogic L G.
+Proof.
+  constructor.
+  apply sepcon_emp.
+Qed.
+
+End OHearnLogic.
+End OHearnLogic.
+
+Module LogicOnModuResModel.
+Section LogicOnModuResModel.
+
+Context (Var: Type).
+
+Instance L: Language := UnitarySeparationLanguage.L Var.
+Instance nL: NormalLanguage L := UnitarySeparationLanguage.nL Var.
+Instance pL: PropositionalLanguage L := UnitarySeparationLanguage.pL Var.
+Instance SL: SeparationLanguage L := UnitarySeparationLanguage.sL Var.
+Instance usL: UnitarySeparationLanguage L := UnitarySeparationLanguage.usL Var.
+
+Inductive provable: expr -> Prop :=
+| modus_ponens: forall x y, provable (x --> y) -> provable x -> provable y
+| axiom1: forall x y, provable (x --> (y --> x))
+| axiom2: forall x y z, provable ((x --> y --> z) --> (x --> y) --> (x --> z))
+| andp_intros: forall x y, provable (x --> y --> x && y)
+| andp_elim1: forall x y, provable (x && y --> x)
+| andp_elim2: forall x y, provable (x && y --> y)
+| orp_intros1: forall x y, provable (x --> x || y)
+| orp_intros2: forall x y, provable (y --> x || y)
+| orp_elim: forall x y z, provable ((x --> z) --> (y --> z) --> (x || y --> z))
+| falsep_elim: forall x, provable (FF --> x)
+| impp_choice: forall x y, provable ((x --> y) || (y --> x))
+| sepcon_comm: forall x y, provable (x * y --> y * x)
+| sepcon_assoc: forall x y z, provable (x * (y * z) <--> (x * y) * z)
+| wand_sepcon_adjoint1: forall x y z, provable (x * y --> z) -> provable (x --> (y -* z))
+| wand_sepcon_adjoint2: forall x y z, provable (x --> (y -* z)) -> provable (x * y --> z)
+| sepcon_mono: forall x1 x2 y1 y2, provable (x1 --> x2) -> provable (y1 --> y2) -> provable ((x1 * y1) --> (x2 * y2))
+| sepcon_emp: forall x, provable (x * emp <--> x)
+| sepcon_elim1: forall x y, provable (x * y --> x).
+
+Instance G: ProofTheory L := Build_AxiomaticProofTheory provable.
+
+Instance nG: NormalProofTheory L G := Build_nAxiomaticProofTheory provable.
+
+Instance mpG: MinimunPropositionalLogic L G.
+Proof.
+  constructor.
+  + apply modus_ponens.
+  + apply axiom1.
+  + apply axiom2.
+Qed.
+
+Instance ipG: IntuitionisticPropositionalLogic L G.
+Proof.
+  constructor.
+  + apply andp_intros.
+  + apply andp_elim1.
+  + apply andp_elim2.
+  + apply orp_intros1.
+  + apply orp_intros2.
+  + apply orp_elim.
+  + apply falsep_elim.
+Qed.
+
+Instance gdpG: GodelDummettPropositionalLogic L G.
+Proof.
+  constructor.
+  apply impp_choice.
+Qed.
+
+Instance sG: SeparationLogic L G.
+Proof.
+  constructor.
+  + apply sepcon_comm.
+  + apply sepcon_assoc.
+  + intros; split.
+    - apply wand_sepcon_adjoint1.
+    - apply wand_sepcon_adjoint2.
+  + apply sepcon_mono.
+Qed.
+
+Instance usG: UnitarySeparationLogic L G.
+Proof.
+  constructor.
+  apply sepcon_emp.
+Qed.
+
+Instance gcsG: GarbageCollectSeparationLogic L G.
+Proof.
+  constructor.
+  apply sepcon_elim1.
+Qed.
+
+End LogicOnModuResModel. 
+End LogicOnModuResModel.
+
+Module LogicOnMSL.
+Section LogicOnMSL.
+
+Context (Var: Type).
+
+Instance L: Language := UnitarySeparationLanguage.L Var.
+Instance nL: NormalLanguage L := UnitarySeparationLanguage.nL Var.
+Instance pL: PropositionalLanguage L := UnitarySeparationLanguage.pL Var.
+Instance SL: SeparationLanguage L := UnitarySeparationLanguage.sL Var.
+Instance usL: UnitarySeparationLanguage L := UnitarySeparationLanguage.usL Var.
+
+Inductive provable: expr -> Prop :=
+| modus_ponens: forall x y, provable (x --> y) -> provable x -> provable y
+| axiom1: forall x y, provable (x --> (y --> x))
+| axiom2: forall x y z, provable ((x --> y --> z) --> (x --> y) --> (x --> z))
+| andp_intros: forall x y, provable (x --> y --> x && y)
+| andp_elim1: forall x y, provable (x && y --> x)
+| andp_elim2: forall x y, provable (x && y --> y)
+| orp_intros1: forall x y, provable (x --> x || y)
+| orp_intros2: forall x y, provable (y --> x || y)
+| orp_elim: forall x y z, provable ((x --> z) --> (y --> z) --> (x || y --> z))
+| falsep_elim: forall x, provable (FF --> x)
+| impp_choice: forall x y, provable ((x --> y) || (y --> x))
+| sepcon_comm: forall x y, provable (x * y --> y * x)
+| sepcon_assoc: forall x y z, provable (x * (y * z) <--> (x * y) * z)
+| wand_sepcon_adjoint1: forall x y z, provable (x * y --> z) -> provable (x --> (y -* z))
+| wand_sepcon_adjoint2: forall x y z, provable (x --> (y -* z)) -> provable (x * y --> z)
+| sepcon_mono: forall x1 x2 y1 y2, provable (x1 --> x2) -> provable (y1 --> y2) -> provable ((x1 * y1) --> (x2 * y2))
+| sepcon_emp: forall x, provable (x * emp <--> x).
+
+Instance G: ProofTheory L := Build_AxiomaticProofTheory provable.
+
+Instance nG: NormalProofTheory L G := Build_nAxiomaticProofTheory provable.
+
+Instance mpG: MinimunPropositionalLogic L G.
+Proof.
+  constructor.
+  + apply modus_ponens.
+  + apply axiom1.
+  + apply axiom2.
+Qed.
+
+Instance ipG: IntuitionisticPropositionalLogic L G.
+Proof.
+  constructor.
+  + apply andp_intros.
+  + apply andp_elim1.
+  + apply andp_elim2.
+  + apply orp_intros1.
+  + apply orp_intros2.
+  + apply orp_elim.
+  + apply falsep_elim.
+Qed.
+
+Instance gdpG: GodelDummettPropositionalLogic L G.
+Proof.
+  constructor.
+  apply impp_choice.
+Qed.
+
+Instance sG: SeparationLogic L G.
+Proof.
+  constructor.
+  + apply sepcon_comm.
+  + apply sepcon_assoc.
+  + intros; split.
+    - apply wand_sepcon_adjoint1.
+    - apply wand_sepcon_adjoint2.
+  + apply sepcon_mono.
+Qed.
+
+Instance usG: UnitarySeparationLogic L G.
+Proof.
+  constructor.
+  apply sepcon_emp.
+Qed.
+
+End LogicOnMSL.
+End LogicOnMSL.
 
